more rel.. and a rule for lists at last

theories/Relational/GenericRulesComplex.v
@@ -142,90 +142,131 @@ Section RelationalProgramLogicFromRelativeMonad.
                 (to_discr (fun a2 => wf2 ⟨πr γ, a2⟩))
                 (to_discr (fun '⟨a1,a2⟩ => wfrel (extend_point γ a1 a2))))∙1 (wmrel γ).
 
-  Definition valid (Γ : Rel) A1 A2
+  Definition MW A1 A2 : Rel :=
+    mkRel (M1 A1 × dfst (W1 A1)) (M2 A2 × dfst (W2 A2))
+          (fun _ _ => dfst (Wrel ⟨A1,A2⟩)).
+
+  Definition progSpec Γ A1 A2 := Γ R==> MW A1 A2.
+
+  Notation prog1 c := (nfst \o πl c).
+  Notation spec1 c := (nsnd \o πl c).
+  Notation prog2 c := (nfst \o πr c).
+  Notation spec2 c := (nsnd \o πr c).
+  Notation specrel c := (πw c).
+  (* Definition prog1 {Γ A1 A2} (c : progSpec Γ A1 A2) := nfst \o πl c. *)
+  (* Definition spec1 {Γ A1 A2} (c : progSpec Γ A1 A2) := nsnd \o πl c. *)
+  (* Definition prog2 {Γ A1 A2} (c : progSpec Γ A1 A2) := nfst \o πr c. *)
+  (* Definition spec2 {Γ A1 A2} (c : progSpec Γ A1 A2) := nsnd \o πr c. *)
+  (* Definition specrel {Γ A1 A2} (c : progSpec Γ A1 A2) := πw c. *)
+
+  Definition mk_progSpec
+             (Γ : Rel) A1 A2
              (c1: πl Γ -> M1 A1) (w1: πl Γ --> W1 A1)
              (c2:πr Γ -> M2 A2) (w2:πr Γ --> W2 A2)
-             (wrel: ⟬Γ⟭ --> Wrel ⟨A1, A2⟩) : SProp :=
-    ((forall γ1 : πl Γ, (θ1 _)∙1 (c1 γ1) ≤  w1 γ1) s/\
-    (forall γ2 : πr Γ, (θ2 _)∙1 (c2 γ2) ≤ w2 γ2) s/\
-    (forall γ : ⟬Γ⟭, θW∙1 ⟨c1 (πl γ), c2 (πr γ)⟩ ≤ wrel γ)).
+             (wrel: ⟬Γ⟭ --> Wrel ⟨A1, A2⟩) : progSpec Γ A1 A2 :=
+    mk_point (Γ R=> MW A1 A2)
+             (fun γl => ⟨c1 γl, w1 γl⟩)
+             (fun γr => ⟨c2 γr, w2 γr⟩)
+             (fun γl γr γw => wrel (mk_point Γ γl γr γw)).
+
+  Definition validity {Γ A1 A2} (c : progSpec Γ A1 A2) : Γ R==> TyRel.
+  Proof.
+    unshelve econstructor.
+    split=> γ /=.
+    exact (Box ((θ1 _)∙1 (prog1 c γ) ≤  spec1 c γ)).
+    exact (Box ((θ2 _)∙1 (prog2 c γ) ≤  spec2 c γ)).
+    move=> /= γl γr γw _ _.
+    exact (Box (θW∙1 ⟨prog1 c γl, prog2 c γr⟩ ≤ specrel c γl γr γw)).
+  Defined.
+
+  Program Definition dArr {Γ} (A : Γ R==> TyRel) : Rel :=
+    mkRel (forall γl : πl Γ, πl A γl) (forall γr : πr Γ, πr A γr)
+          (fun fl fr => forall γl γr γw, πw A γl γr γw (fl γl) (fr γr)).
+
+  Definition valid Γ {A1 A2} (c : progSpec Γ A1 A2) := ⟬dArr (validity c)⟭.
+
+  Notation " Γ ⊫ c1 ≈ c2 [{ w1 , w2 , w }] " :=
+    (valid Γ (mk_progSpec Γ _ _ c1 w1 c2 w2 w)).
+
 
   Definition retWrel {A1 A2} : A1 -> A2 --> Wrel ⟨A1,A2⟩ :=
     fun a1 a2 => (rsmc_return Wrel ⟨A1,A2⟩)∙1 ⟨a1, a2⟩.
 
   Definition retW {W : unarySpecMonad} {A} : A --> W A := (ord_relmon_unit W A)∙1.
 
-  Lemma ValidRet Γ A1 A2 a1 a2:
-    valid Γ A1 A2  (ret \o a1)  (retW \o a1) (ret \o a2) (retW \o a2)
-          (fun γ => retWrel (a1 (πl γ)) (a2 (πr γ))).
+  Ltac destruct_valid :=
+    unshelve econstructor; [split=> /= γ|move=> /= γl γr γw]; constructor.
+
+  Lemma ValidRet Γ A1 A2 (a1: _ -> A1) (a2 : _ -> A2) :
+    Γ ⊫ ret \o a1 ≈ ret \o a2 [{retW \o a1, retW \o a2, (fun γ => retWrel (a1 (πl γ)) (a2 (πr γ)))}].
   Proof.
-    split;[split|]=> γ.
+    destruct_valid.
     - move: (rmm_law1 _ _ _ _ θ1 A1) => /(f_equal (fun f=> f∙1 (a1 γ))) /= ->.
       sreflexivity.
     - move: (rmm_law1 _ _ _ _ θ2 A2) => /(f_equal (fun f=> f∙1 (a2 γ))) /= ->.
       sreflexivity.
     - move: (@reoc_law1 _ _ _ _ _ _ _ θrc ⟨A1,A2⟩)
-      => /(f_equal (fun f=> f∙1 ⟨a1 (πl γ), a2 (πr γ)⟩)) /= ->.
+      => /(f_equal (fun f=> f∙1 ⟨a1 γl, a2 γr⟩)) /= ->.
       sreflexivity.
   Qed.
-
 
   Definition bindWStr {W : unarySpecMonad} {Γ A B}
              (wm: Γ --> W A) (wf : Γ × A --> W B) : Γ --> W B :=
     fun γ => (ord_relmon_bind W (to_discr (fun a => wf⟨γ, a⟩)))∙1 (wm γ).
 
   Lemma ValidBind
-        Γ A1 A2 B1 B2 m1 wm1 m2 wm2 wmrel f1 wf1 f2 wf2 wfrel :
-    valid Γ A1 A2 m1 wm1 m2 wm2 wmrel ->
-    valid (extends Γ A1 A2) B1 B2 f1 wf1 f2 wf2 wfrel ->
-    valid Γ B1 B2
-          (bindStr m1 f1) (bindWStr wm1 wf1)
-          (bindStr m2 f2) (bindWStr wm2 wf2)
-          (bindWrelStrong wm1 wm2 wmrel wf1 wf2 wfrel).
+        Γ A1 A2 B1 B2 m1 wm1 m2 wm2 wmrel
+        (f1: _ × A1 -> M1 B1) wf1 (f2: _ × A2 -> M2 B2) wf2 wfrel :
+    Γ ⊫ m1 ≈ m2 [{ wm1,  wm2, wmrel }] ->
+    extends Γ A1 A2 ⊫ f1 ≈ f2 [{wf1, wf2, wfrel}] ->
+    Γ ⊫ bindStr m1 f1 ≈ bindStr m2 f2
+      [{bindWStr wm1 wf1,
+        bindWStr wm2 wf2,
+        bindWrelStrong wm1 wm2 wmrel wf1 wf2 wfrel}].
   Proof.
-    move=> [[Hm1 Hm2] Hm] [[Hf1 Hf2] Hf].
-    split; [split|]=> γ.
+    move=> [[/= Hm1 Hm2] Hm] [[/= Hf1 Hf2] Hf].
+    destruct_valid.
     - move: (rmm_law2 _ _ _ _ θ1 _ _ (fun a => f1 ⟨γ,a⟩))
       => /(f_equal (fun f=> f∙1 (m1 γ))) /= ->.
-      apply: ordCat_helper; last by apply: Hm1.
-      apply: (ord_relmon_bind_proper W1)=> ? ; apply: Hf1.
+      apply: ordCat_helper; last by apply: (unbox (Hm1 _)).
+      apply: (ord_relmon_bind_proper W1)=> ? ; apply: (unbox (Hf1 _)).
     - move: (rmm_law2 _ _ _ _ θ2 _ _ (fun a=> f2 ⟨γ,a⟩))
       => /(f_equal (fun f=> f∙1 (m2 γ))) /= ->.
-      apply: ordCat_helper; last by apply: Hm2.
-      apply: (ord_relmon_bind_proper W2)=> ?; apply: Hf2.
-    - move: (reoc_law2 _ _ _ _ _ θrc (to_prod (fun a=> f1 ⟨πl γ,a⟩) (fun a=> f2 ⟨πr γ,a⟩))) => /=.
-      move=> /(f_equal (fun f=> f∙1 ⟨m1 (πl γ),m2 (πr γ)⟩)) /= ->; estransitivity;
-      last (eapply ((actW _ _ _)∙2)=> //; apply (Hm ⦑tt,tt|I⦒)).
+      apply: ordCat_helper; last by apply: (unbox (Hm2 _)).
+      apply: (ord_relmon_bind_proper W2)=> ?; apply: (unbox (Hf2 _)).
+    - move: (reoc_law2 _ _ _ _ _ θrc (to_prod (fun a=> f1 ⟨γl,a⟩) (fun a=> f2 ⟨γr,a⟩))) => /=.
+      move=> /(f_equal (fun f=> f∙1 ⟨m1 γl,m2 γr⟩)) /= ->; estransitivity;
+              last (eapply ((actW _ _ _)∙2)=> //; apply (unbox (Hm _ _ _))).
       apply: rsmc_act_proper;
-        [move=> ? ; apply: Hf1| move=> ?; apply: Hf2|].
-      move=> [? ?] /=; set γ' := extend_point _ _ _; apply: (Hf γ').
+        [move=> ? ; apply: (unbox (Hf1 _))| move=> ?; apply: (unbox (Hf2 _))|].
+      move=> [? ?] /=; apply: (unbox (Hf _ _ _)).
   Qed.
 
   Notation "x ⩿ y" := (pointwise_srelation _ (@extract_ord _) x y) (at level 70).
 
   Lemma ValidWeaken
-             Γ A1 A2 m1 wm1 wm1' m2 wm2 wm2' wmrel wmrel':
-    valid Γ A1 A2 m1 wm1 m2 wm2 wmrel ->
+        Γ A1 A2 (m1 : _ -> M1 A1) wm1 wm1'
+        (m2: _ -> M2 A2) wm2 wm2' wmrel wmrel':
+    Γ ⊫ m1 ≈ m2 [{ wm1, wm2, wmrel}] ->
     wm1 ⩿ wm1' -> wm2 ⩿ wm2' -> wmrel ⩿ wmrel' ->
-    valid Γ A1 A2 m1 wm1' m2 wm2' wmrel'.
+    Γ ⊫ m1 ≈ m2 [{ wm1', wm2', wmrel'}].
   Proof.
-    move=> [[H1 H2] H] Hle1 Hle2 Hle; split; [split|] => ?; estransitivity.
-    apply: H1. apply: Hle1.
-    apply: H2. apply: Hle2.
-    apply: H. apply: Hle.
+    move=> [[/= H1 H2] H] Hle1 Hle2 Hle; destruct_valid ; estransitivity.
+    apply: (unbox (H1 _)). apply: Hle1.
+    apply: (unbox (H2 _)). apply: Hle2.
+    apply: (unbox (H _ _ _))=>//. apply: Hle.
   Qed.
 
-  Lemma ValidSubst Γ Δ A1 A2 m1 wm1 m2 wm2 wmrel (σ: Δ R==> Γ) :
-    valid Γ A1 A2 m1 wm1 m2 wm2 wmrel ->
-    valid Δ A1 A2
-          (m1 \o πl σ) (wm1 \o πl σ)
-          (m2 \o πr σ) (wm2 \o πr σ)
-          (wmrel \o applyRel _ _ σ).
+  Lemma ValidSubst Γ Δ A1 A2 (m1: _ -> M1 A1) wm1
+        (m2: _ -> M2 A2) wm2 wmrel (σ: Δ R==> Γ) :
+    Γ ⊫ m1 ≈ m2 [{ wm1, wm2, wmrel}] ->
+    Δ ⊫ m1 \o πl σ ≈ m2 \o πr σ
+      [{ wm1 \o πl σ, wm2 \o πr σ, wmrel \o applyRel _ _ σ}].
   Proof.
-    move=> [[H1 H2] H]; split; [split|]=> γ.
-    apply: H1.
-    apply: H2.
-    set γ' := (σ @R γ); exact: (H γ').
+    move=> [[/= H1 H2] H]; destruct_valid.
+    apply: (unbox (H1 _)).
+    apply: (unbox (H2 _)).
+    apply: (unbox (H _ _ _)).
   Qed.
 
   Definition subst_true {Γ} : Γ -> Γ × bool := fun γ => ⟨γ, true⟩.
@@ -238,33 +279,262 @@ Section RelationalProgramLogicFromRelativeMonad.
   Definition extend_Lo {Γ A} (γ:⟬Γ⟭) (a1 a2 : A) (H : a1 = a2) : ⟬Γ,∙A⟭ :=
     mk_point (Γ,∙A) ⟨πl γ,a1⟩ ⟨πr γ, a2⟩ ⟨πw γ, H⟩.
 
-  Lemma ValidBoolElim Γ A1 A2 m1 wm1 m2 wm2 wmrel:
-    valid Γ A1 A2 (m1 \o subst_true) (wm1 \o subst_true)
-          (m2 \o subst_true) (wm2 \o subst_true) (wmrel \o rel_subst_true) ->
-    valid Γ A1 A2 (m1 \o subst_false) (wm1 \o subst_false)
-          (m2 \o subst_false) (wm2 \o subst_false) (wmrel \o rel_subst_false) ->
-      valid (Γ ,∙ bool) A1 A2 m1 wm1 m2 wm2 wmrel.
+  Lemma ValidBoolElim Γ A1 A2 (m1: _ -> M1 A1) wm1 (m2: _ -> M2 A2) wm2 wmrel:
+    Γ ⊫ m1 \o subst_true ≈ m2 \o subst_true
+      [{wm1 \o subst_true, wm2 \o subst_true, wmrel \o rel_subst_true}] ->
+    Γ ⊫ m1 \o subst_false ≈ m2 \o subst_false
+      [{wm1 \o subst_false, wm2 \o subst_false, wmrel \o rel_subst_false}] ->
+    (Γ,∙ bool) ⊫ m1 ≈ m2 [{ wm1, wm2, wmrel}].
   Proof.
-    move=> [[Ht1 Ht2] Ht] [[Hf1 Hf2] Hf]; split; [split|].
-    move=> [γ []]; [apply Ht1| apply Hf1].
-    move=> [γ []]; [apply Ht2| apply Hf2].
-    move=> [[[γ1 []] [γ2 b2]] [γ b]] /= ;
+    move=> [[/= Ht1 Ht2] Ht] [[/= Hf1 Hf2] Hf]; destruct_valid.
+    move: γ => [γ []]; [apply (unbox (Ht1 _))| apply (unbox (Hf1 _))].
+    move: γ => [γ []]; [apply (unbox (Ht2 _))| apply (unbox (Hf2 _))].
+    move: γl γr γw => [γ1 []] [γ2 b2] /= [γ b] ;
     pattern b2, b;
     match goal with
     | [|- ?g _ _] =>
       refine (match b as Hb in _ = b' return g b' Hb with | erefl => _ end)
     end;
-    set γ' := mk_point _ γ1 γ2 γ.
-    exact: (Ht γ').
-    exact: (Hf γ').
+    [apply: (unbox (Ht _ _ _))| apply: (unbox (Hf _ _ _))].
   Qed.
-    (* rewrite /rel_subst_true /extend_Lo /mk_point /subst_true /applyRel /=. *)
-    (* trivial. *)
-    (* simpl. *)
-    (* unfold rel_subst_true, extend_Lo. *)
-    (* simpl. *)
-    (* apply Ht. *)
-    (* set γ0 := ⦑ _ ⦒. *)
+
+
+  Definition subst_nil {Γ A} : Γ -> Γ × list A := fun γ => ⟨γ, nil⟩.
+
+  Definition rel_subst_nil {Γ A} : ⟬Γ⟭ -> ⟬Γ ,∙ list A⟭ :=
+    fun γ => mk_point (Γ ,∙ list A) (subst_nil (πl γ)) (subst_nil (πr γ))
+                  ⟨πw γ, eq_refl⟩.
+
+  Definition subst_cons {Γ A} : Γ × A × list A -> Γ × list A :=
+    fun γal => ⟨nfst (nfst γal), cons (nsnd (nfst γal)) (nsnd γal)⟩.
+
+  Program Definition rel_subst_cons {Γ A} : ⟬Γ,∙A,∙list A⟭ -> ⟬Γ ,∙ list A⟭ :=
+    fun γ => mk_point (Γ ,∙ list A) (subst_cons (πl γ)) (subst_cons (πr γ))
+                  ⟨nfst (nfst (πw γ)), eq_refl⟩.
+  Next Obligation. move: γ=> [? [[?]]] /= -> -> //. Defined.
+
+  Definition ctx_subst_extend {A Γ' Γ} (σ: Γ' R==> Γ) : (Γ' ,∙ A) R==> (Γ ,∙ A)
+    :=
+      mk_point ((Γ' ,∙ A) R=> (Γ ,∙ A)) (fun e => ⟨(πl σ) (nfst e), nsnd e⟩)
+               (fun e => ⟨(πr σ) (nfst e), nsnd e⟩) (fun xl xr X => ⟨(πw σ) (nfst xl) (nfst xr) (nfst X), nsnd X⟩).
+
+  Program Definition weaken_subst {Γ A B} : (Γ,∙A,∙B) R==> (Γ,∙B) :=
+    mk_point ((Γ,∙A,∙B) R=> (Γ,∙B))
+             (fun '⟨⟨γ,_⟩,b⟩ => ⟨γ,b⟩)
+             (fun '⟨⟨γ,_⟩,b⟩ => ⟨γ,b⟩)
+             (fun _ _ '⟨⟨γ,_⟩,b⟩ => ⟨γ,b⟩).
+
+  Program Definition dArrCtx {Γ} (A B : Γ R==> TyRel) : Rel :=
+    mkRel (forall γl : πl Γ, πl A γl -> πl B γl)
+          (forall γr : πr Γ, πr A γr -> πr B γr)
+          (fun fl fr => forall γl γr γw al ar,
+               πw A γl γr γw al ar ->
+               πw B γl γr γw (fl γl al) (fr γr ar)).
+
+  Tactic Notation "destruct_valid_pat"
+         simple_intropattern(γl)
+         simple_intropattern(γr)
+         simple_intropattern(γw) :=
+    unshelve econstructor; [split=> /= [γl|γr]|move=> /= γl γr γw]; constructor.
+
+  Lemma ValidListElim Γ A A1 A2 (m1: _ -> M1 A1) wm1 (m2: _ -> M2 A2) wm2 wmrel :
+    Γ ⊫ m1 \o subst_nil ≈ m2 \o subst_nil
+      [{wm1 \o subst_nil, wm2 \o subst_nil, wmrel \o rel_subst_nil}] ->
+    ⟬dArrCtx (compRel weaken_subst
+                      (validity (mk_progSpec (Γ,∙list A) _ _ m1 wm1 m2 wm2 wmrel)))
+             (validity (mk_progSpec (Γ,∙A,∙list A) _ _
+                                    (m1 \o subst_cons) (wm1 \o subst_cons)
+                                    (m2 \o subst_cons) (wm2 \o subst_cons)
+                                    (wmrel \o rel_subst_cons)))⟭ ->
+    (Γ,∙ list A) ⊫ m1 ≈ m2 [{ wm1, wm2, wmrel}].
+  Proof.
+    move=> [[/= Hnil1 Hnil2] Hnil] [[/= Hcons1 Hcons2] Hcons].
+    (* destruct_valid_pat [γl ll] [γr lr] [γw lw]. *)
+    destruct_valid.
+    - move: γ => [?] ; elim.
+      + apply: (unbox (Hnil1 _)).
+      + move=> ? ? ?; apply: (unbox (Hcons1 ⟨⟨_, _⟩, _⟩ (box _)))=> //.
+    - move: γ => [?] ; elim.
+      + apply: (unbox (Hnil2 _)).
+      + move=> ? ? ?; apply: (unbox (Hcons2 ⟨⟨_, _⟩, _⟩ (box _)))=> //.
+    - match goal with
+      | [|- ?G ] =>
+        enough ((θ1 _ )∙1 (m1 γl) ≤ wm1 γl s/\
+                (θ2 _ )∙1 (m2 γr) ≤ wm2 γr s/\ G) as [[]]=> //
+      end.
+      move: γl γr γw=> [γl ll] [γr lr] [/= γw] ;
+                        elim: ll lr=> [|xl xls /(fun f => f xls erefl) [[? ?] ?]];
+      match goal with
+      | [|- forall lr lw, @?G lr lw ] =>
+        refine (fun lr lw => match lw as Heq in _ = l return G l Heq with
+                          | erefl => _ end)
+      end; split; try split.
+      apply: (unbox (Hnil1 _)).
+      apply: (unbox (Hnil2 _)).
+      apply: (unbox (Hnil _ _ _)).
+
+      apply: (unbox (Hcons1 ⟨⟨_, _⟩, _⟩ (box _)))=> //.
+      apply: (unbox (Hcons2 ⟨⟨_, _⟩, _⟩ (box _)))=> //.
+      apply: (unbox (Hcons ⟨⟨γl, xl⟩, xls⟩ ⟨⟨γr, xl⟩, xls⟩ ⟨⟨γw, erefl⟩, erefl⟩ (box _) (box _) (box _)))=> //.
+  Qed.
+
+
+
+  (* Definition valid {Γ A1 A2} (c : progSpec Γ A1 A2) : Rel := *)
+  (*   mkRel (Box (forall γ1 : πl Γ, (θ1 _)∙1 (prog1 c γ1) ≤  spec1 c γ1)) *)
+  (*         (Box (forall γ2 : πr Γ, (θ2 _)∙1 (prog2 c γ2) ≤ spec2 c γ2)) *)
+  (*         (fun _ _ => Box (forall γ : ⟬Γ⟭, θW∙1 ⟨prog1 c (πl γ), prog2 c (πr γ)⟩ ≤ specrel c (πl γ) (πr γ) (πw γ))). *)
+
+  (* Definition valid (Γ : Rel) A1 A2 *)
+  (*            (c1: πl Γ -> M1 A1) (w1: πl Γ --> W1 A1) *)
+  (*            (c2:πr Γ -> M2 A2) (w2:πr Γ --> W2 A2) *)
+  (*            (wrel: ⟬Γ⟭ --> Wrel ⟨A1, A2⟩) : SProp := *)
+  (*   ((forall γ1 : πl Γ, (θ1 _)∙1 (c1 γ1) ≤  w1 γ1) s/\ *)
+  (*   (forall γ2 : πr Γ, (θ2 _)∙1 (c2 γ2) ≤ w2 γ2) s/\ *)
+  (*   (forall γ : ⟬Γ⟭, θW∙1 ⟨c1 (πl γ), c2 (πr γ)⟩ ≤ wrel γ)). *)
+
+  (* Definition retWrel {A1 A2} : A1 -> A2 --> Wrel ⟨A1,A2⟩ := *)
+  (*   fun a1 a2 => (rsmc_return Wrel ⟨A1,A2⟩)∙1 ⟨a1, a2⟩. *)
+
+  (* Definition retW {W : unarySpecMonad} {A} : A --> W A := (ord_relmon_unit W A)∙1. *)
+
+  (* Lemma ValidRet Γ A1 A2 a1 a2: *)
+  (*   valid Γ A1 A2  (ret \o a1)  (retW \o a1) (ret \o a2) (retW \o a2) *)
+  (*         (fun γ => retWrel (a1 (πl γ)) (a2 (πr γ))). *)
+  (* Proof. *)
+  (*   split;[split|]=> γ. *)
+  (*   - move: (rmm_law1 _ _ _ _ θ1 A1) => /(f_equal (fun f=> f∙1 (a1 γ))) /= ->. *)
+  (*     sreflexivity. *)
+  (*   - move: (rmm_law1 _ _ _ _ θ2 A2) => /(f_equal (fun f=> f∙1 (a2 γ))) /= ->. *)
+  (*     sreflexivity. *)
+  (*   - move: (@reoc_law1 _ _ _ _ _ _ _ θrc ⟨A1,A2⟩) *)
+  (*     => /(f_equal (fun f=> f∙1 ⟨a1 (πl γ), a2 (πr γ)⟩)) /= ->. *)
+  (*     sreflexivity. *)
+  (* Qed. *)
+
+
+  (* Definition bindWStr {W : unarySpecMonad} {Γ A B} *)
+  (*            (wm: Γ --> W A) (wf : Γ × A --> W B) : Γ --> W B := *)
+  (*   fun γ => (ord_relmon_bind W (to_discr (fun a => wf⟨γ, a⟩)))∙1 (wm γ). *)
+
+  (* Lemma ValidBind *)
+  (*       Γ A1 A2 B1 B2 m1 wm1 m2 wm2 wmrel f1 wf1 f2 wf2 wfrel : *)
+  (*   valid Γ A1 A2 m1 wm1 m2 wm2 wmrel -> *)
+  (*   valid (extends Γ A1 A2) B1 B2 f1 wf1 f2 wf2 wfrel -> *)
+  (*   valid Γ B1 B2 *)
+  (*         (bindStr m1 f1) (bindWStr wm1 wf1) *)
+  (*         (bindStr m2 f2) (bindWStr wm2 wf2) *)
+  (*         (bindWrelStrong wm1 wm2 wmrel wf1 wf2 wfrel). *)
+  (* Proof. *)
+  (*   move=> [[Hm1 Hm2] Hm] [[Hf1 Hf2] Hf]. *)
+  (*   split; [split|]=> γ. *)
+  (*   - move: (rmm_law2 _ _ _ _ θ1 _ _ (fun a => f1 ⟨γ,a⟩)) *)
+  (*     => /(f_equal (fun f=> f∙1 (m1 γ))) /= ->. *)
+  (*     apply: ordCat_helper; last by apply: Hm1. *)
+  (*     apply: (ord_relmon_bind_proper W1)=> ? ; apply: Hf1. *)
+  (*   - move: (rmm_law2 _ _ _ _ θ2 _ _ (fun a=> f2 ⟨γ,a⟩)) *)
+  (*     => /(f_equal (fun f=> f∙1 (m2 γ))) /= ->. *)
+  (*     apply: ordCat_helper; last by apply: Hm2. *)
+  (*     apply: (ord_relmon_bind_proper W2)=> ?; apply: Hf2. *)
+  (*   - move: (reoc_law2 _ _ _ _ _ θrc (to_prod (fun a=> f1 ⟨πl γ,a⟩) (fun a=> f2 ⟨πr γ,a⟩))) => /=. *)
+  (*     move=> /(f_equal (fun f=> f∙1 ⟨m1 (πl γ),m2 (πr γ)⟩)) /= ->; estransitivity; *)
+  (*     last (eapply ((actW _ _ _)∙2)=> //; apply (Hm ⦑tt,tt|I⦒)). *)
+  (*     apply: rsmc_act_proper; *)
+  (*       [move=> ? ; apply: Hf1| move=> ?; apply: Hf2|]. *)
+  (*     move=> [? ?] /=; set γ' := extend_point _ _ _; apply: (Hf γ'). *)
+  (* Qed. *)
+
+  (* Notation "x ⩿ y" := (pointwise_srelation _ (@extract_ord _) x y) (at level 70). *)
+
+  (* Lemma ValidWeaken *)
+  (*            Γ A1 A2 m1 wm1 wm1' m2 wm2 wm2' wmrel wmrel': *)
+  (*   valid Γ A1 A2 m1 wm1 m2 wm2 wmrel -> *)
+  (*   wm1 ⩿ wm1' -> wm2 ⩿ wm2' -> wmrel ⩿ wmrel' -> *)
+  (*   valid Γ A1 A2 m1 wm1' m2 wm2' wmrel'. *)
+  (* Proof. *)
+  (*   move=> [[H1 H2] H] Hle1 Hle2 Hle; split; [split|] => ?; estransitivity. *)
+  (*   apply: H1. apply: Hle1. *)
+  (*   apply: H2. apply: Hle2. *)
+  (*   apply: H. apply: Hle. *)
+  (* Qed. *)
+
+  (* Lemma ValidSubst Γ Δ A1 A2 m1 wm1 m2 wm2 wmrel (σ: Δ R==> Γ) : *)
+  (*   valid Γ A1 A2 m1 wm1 m2 wm2 wmrel -> *)
+  (*   valid Δ A1 A2 *)
+  (*         (m1 \o πl σ) (wm1 \o πl σ) *)
+  (*         (m2 \o πr σ) (wm2 \o πr σ) *)
+  (*         (wmrel \o applyRel _ _ σ). *)
+  (* Proof. *)
+  (*   move=> [[H1 H2] H]; split; [split|]=> γ. *)
+  (*   apply: H1. *)
+  (*   apply: H2. *)
+  (*   set γ' := (σ @R γ); exact: (H γ'). *)
+  (* Qed. *)
+
+  (* Definition subst_true {Γ} : Γ -> Γ × bool := fun γ => ⟨γ, true⟩. *)
+  (* Definition rel_subst_true {Γ} : ⟬Γ⟭ -> ⟬Γ,∙bool ⟭ := *)
+  (*   applyRel _ _ (mk_point (Γ R=> (Γ,∙bool)) subst_true subst_true (fun _ _ γ => ⟨γ, erefl⟩)). *)
+  (* Definition subst_false {Γ} : Γ -> Γ × bool := fun γ => ⟨γ, false⟩. *)
+  (* Definition rel_subst_false {Γ} : ⟬Γ⟭ -> ⟬Γ,∙bool ⟭ := *)
+  (*   applyRel _ _ (mk_point (Γ R=> (Γ,∙bool)) subst_false subst_false (fun _ _ γ => ⟨γ, erefl⟩)). *)
+
+  (* Definition extend_Lo {Γ A} (γ:⟬Γ⟭) (a1 a2 : A) (H : a1 = a2) : ⟬Γ,∙A⟭ := *)
+  (*   mk_point (Γ,∙A) ⟨πl γ,a1⟩ ⟨πr γ, a2⟩ ⟨πw γ, H⟩. *)
+
+  (* Lemma ValidBoolElim Γ A1 A2 m1 wm1 m2 wm2 wmrel: *)
+  (*   valid Γ A1 A2 (m1 \o subst_true) (wm1 \o subst_true) *)
+  (*         (m2 \o subst_true) (wm2 \o subst_true) (wmrel \o rel_subst_true) -> *)
+  (*   valid Γ A1 A2 (m1 \o subst_false) (wm1 \o subst_false) *)
+  (*         (m2 \o subst_false) (wm2 \o subst_false) (wmrel \o rel_subst_false) -> *)
+  (*     valid (Γ ,∙ bool) A1 A2 m1 wm1 m2 wm2 wmrel. *)
+  (* Proof. *)
+  (*   move=> [[Ht1 Ht2] Ht] [[Hf1 Hf2] Hf]; split; [split|]. *)
+  (*   move=> [γ []]; [apply Ht1| apply Hf1]. *)
+  (*   move=> [γ []]; [apply Ht2| apply Hf2]. *)
+  (*   move=> [[[γ1 []] [γ2 b2]] [γ b]] /= ; *)
+  (*   pattern b2, b; *)
+  (*   match goal with *)
+  (*   | [|- ?g _ _] => *)
+  (*     refine (match b as Hb in _ = b' return g b' Hb with | erefl => _ end) *)
+  (*   end; *)
+  (*   set γ' := mk_point _ γ1 γ2 γ. *)
+  (*   exact: (Ht γ'). *)
+  (*   exact: (Hf γ'). *)
+  (* Qed. *)
+
+  (* Definition subst_nil {Γ A} : Γ -> Γ × list A := fun γ => ⟨γ, nil⟩. *)
+
+  (* Definition rel_subst_nil {Γ A} : ⟬Γ⟭ -> ⟬Γ ,∙ list A⟭ := *)
+  (*   fun γ => mk_point (Γ ,∙ list A) (subst_nil (πl γ)) (subst_nil (πr γ)) *)
+  (*                 ⟨πw γ, eq_refl⟩. *)
+
+  (* Definition subst_cons {Γ A} : Γ × A × list A -> Γ × list A := *)
+  (*   fun γal => ⟨nfst (nfst γal), cons (nsnd (nfst γal)) (nsnd γal)⟩. *)
+
+  (* Program Definition rel_subst_cons {Γ A} : ⟬Γ,∙A,∙list A⟭ -> ⟬Γ ,∙ list A⟭ := *)
+  (*   fun γ => mk_point (Γ ,∙ list A) (subst_cons (πl γ)) (subst_cons (πr γ)) *)
+  (*                 ⟨nfst (nfst (πw γ)), eq_refl⟩. *)
+  (* Next Obligation. move: γ=> [? [[?]]] /= -> -> //. Qed. *)
+
+  (* Definition ctx_subst_extend {A Γ' Γ} (σ: Γ' R==> Γ) : (Γ' ,∙ A) R==> (Γ ,∙ A) *)
+  (*   := *)
+  (*     mk_point ((Γ' ,∙ A) R=> (Γ ,∙ A)) (fun e => ⟨(πl σ) (nfst e), nsnd e⟩) *)
+  (*              (fun e => ⟨(πr σ) (nfst e), nsnd e⟩) (fun xl xr X => ⟨(πw σ) (nfst xl) (nfst xr) (nfst X), nsnd X⟩). *)
+
+  (* Lemma ValidListElim Γ A A1 A2 m1 wm1 m2 wm2 wmrel : *)
+  (*   valid Γ A1 A2 *)
+  (*         (m1 \o subst_nil) (wm1 \o subst_nil) *)
+  (*         (m2 \o subst_nil) (wm2 \o subst_nil) *)
+  (*         (wmrel \o rel_subst_nil) -> *)
+  (*   (valid (Γ,∙ list A) A1 A2 m1 wm1 m2 wm2 wmrel -> *)
+  (*    valid (Γ,∙ A ,∙ list A) A1 A2 *)
+  (*          (m1 \o subst_cons) (wm1 \o subst_cons) *)
+  (*          (m2 \o subst_cons) (wm2 \o subst_cons) *)
+  (*          (wmrel \o rel_subst_cons)) -> *)
+  (*   valid (Γ,∙ list A) A1 A2 m1 wm1 m2 wm2 wmrel. *)
+  (* Proof. *)
+  (*   move=> [[Hnil1 Hnil2] Hnil] Hcons ; split; [split|]. *)
+
 
   (* Definition bindStrongRSM {Γ A1 A2 B1 B2} *)
   (*            (wm1 : πl Γ -> W1 A1) *)
